use Frakturs for TYPE

theories/prophecy/prophecy.v
@@ -13,17 +13,17 @@ Ltac proof_subst x y :=
 Section basic.
 Context `{!EqDecision TYPE} {Ty: TYPE → Type}.
 Coercion Ty: TYPE >-> Sortclass.
-Implicit Type a b: TYPE.
+Implicit Type 𝔄 𝔅: TYPE.
 
 (** * Basic Notions *)
 
-Definition proph_var_body a : Type := positive * inhabited a.
+Definition proph_var_body 𝔄 : Type := positive * inhabited 𝔄.
 Record proph_var := PrVar { pv_ty: TYPE; pv_bd: proph_var_body pv_ty }.
 Add Printing Constructor proph_var.
 
 Global Instance proph_var_eq_dec: EqDecision proph_var.
 Proof.
-  move=> [a[i inh]][b[j inh']]. case (decide (a = b))=> [?|?];
+  move=> [𝔄[i inh]][𝔅[j inh']]. case (decide (𝔄 = 𝔅))=> [?|?];
   [|by apply right=> [=]]. subst. case (decide (i = j))=> [?|?].
   - subst. apply left. by proof_subst inh inh'.
   - apply right=> Eq. by dependent destruction Eq.
@@ -156,15 +156,15 @@ Qed.
 
 (** * Prophecy Camera *)
 
-Local Definition proph_itemR a := csumR fracR (agreeR (leibnizO (proph a))).
-Local Definition proph_gmapUR a := gmapUR positive (proph_itemR a).
+Local Definition proph_itemR 𝔄 := csumR fracR (agreeR (leibnizO (proph 𝔄))).
+Local Definition proph_gmapUR 𝔄 := gmapUR positive (proph_itemR 𝔄).
 Local Definition proph_smryUR := discrete_funUR proph_gmapUR.
 Definition prophUR := authUR proph_smryUR.
 
 Implicit Type (S: proph_smryUR) (q: Qp).
 
-Local Definition aitem {a} vπ : proph_itemR a := Cinr (to_agree vπ).
-Local Definition fitem {a} q : proph_itemR a := Cinl q.
+Local Definition aitem {𝔄} vπ : proph_itemR 𝔄 := Cinr (to_agree vπ).
+Local Definition fitem {𝔄} q : proph_itemR 𝔄 := Cinl q.
 Local Definition line ξ it : proph_smryUR := .{[ξ.(pv_ty) := {[ξ.(pv_bd).1 := it]}]}.
 Local Definition add_line ξ it S : proph_smryUR :=
   .<[ξ.(pv_ty) := <[ξ.(pv_bd).1 := it]> (S ξ.(pv_ty))]> S.
@@ -229,7 +229,7 @@ Local Notation "S :~ L" := (proph_sim S L) (at level 70, format "S  :~  L").
 Section lemmas.
 Context `{!invG Σ, !prophG TYPE Ty Σ}.
 Coercion Ty: TYPE >-> Sortclass.
-Implicit Type a b: TYPE.
+Implicit Type 𝔄 𝔅: TYPE.
 
 (** Instances *)
 
@@ -286,22 +286,22 @@ Proof.
   rewrite lookup_empty. split=> Hyp; inversion Hyp.
 Qed.
 
-(** Taking a Fresh Prophecy Variable *)
+(** Taking 𝔄 Fresh Prophecy Variable *)
 
-Lemma proph_intro a (I: gset positive) E (inh: inhabited a) :
-  ↑prophN ⊆ E → proph_ctx ={E}=∗ ∃i, ⌜i ∉ I⌝ ∗ 1:[PrVar a (i, inh)].
+Lemma proph_intro 𝔄 (I: gset positive) E (inh: inhabited 𝔄) :
+  ↑prophN ⊆ E → proph_ctx ={E}=∗ ∃i, ⌜i ∉ I⌝ ∗ 1:[PrVar 𝔄 (i, inh)].
 Proof.
   iIntros (?) "?". iInv prophN as (S) "> [(%L & %Ok & %Sim) Auth]".
-  case (exist_fresh (I ∪ dom _ (S a)))
+  case (exist_fresh (I ∪ dom _ (S 𝔄)))
     => [i /not_elem_of_union [? /not_elem_of_dom EqNone]].
-  set ξ := PrVar a (i, inh). set S' := add_line ξ (fitem 1) S.
+  set ξ := PrVar 𝔄 (i, inh). set S' := add_line ξ (fitem 1) S.
   iMod (own_update _ _ (● S' ⋅ ◯ line ξ (fitem 1)) with "Auth") as "[Auth ?]".
   { by apply auth_update_alloc,
       discrete_fun_insert_local_update, alloc_singleton_local_update. }
   iModIntro. iSplitL "Auth"; last first. { iModIntro. iExists i. by iFrame. }
   iModIntro. iExists S'. iFrame. iPureIntro. exists L.
-  split; [done|]. case=> [b[j ?]]?. rewrite /S' /add_line /discrete_fun_insert -Sim.
-  case (decide (a = b))=> [?|?]; [|done]. subst=>/=.
+  split; [done|]. case=> [𝔅[j ?]]?. rewrite /S' /add_line /discrete_fun_insert -Sim.
+  case (decide (𝔄 = 𝔅))=> [?|?]; [|done]. subst=>/=.
   case (decide (i = j))=> [<-|?]; [|by rewrite lookup_insert_ne].
   rewrite lookup_insert EqNone. split=> Eqv; [apply (inj Some) in Eqv|]; inversion Eqv.
 Qed.
@@ -313,9 +313,9 @@ Local Lemma proph_tok_out S L ξ q :
 Proof.
   move=> Sim. iIntros "Auth Tok".
   iDestruct (own_valid_2 with "Auth Tok") as %ValBoth. iPureIntro.
-  move=> /(elem_of_list_fmap_2 pli_pv) [[[a[i ?]]?][? /Sim Eqv]]. simpl in *.
+  move=> /(elem_of_list_fmap_2 pli_pv) [[[𝔄[i ?]]?][? /Sim Eqv]]. simpl in *.
   subst. move: ValBoth=> /auth_both_valid_discrete [Inc _].
-  move/(discrete_fun_included_spec_1 _ _ a) in Inc.
+  move/(discrete_fun_included_spec_1 _ _ 𝔄) in Inc.
   rewrite /line discrete_fun_lookup_singleton /= in Inc.
   move: Eqv. move: Inc=> /singleton_included_l [?[-> Inc]]. move=> Eqv.
   apply (inj Some) in Eqv. move: Inc. rewrite Eqv.
@@ -334,7 +334,7 @@ Qed.
 Lemma proph_resolve E ξ vπ ζs q : ↑prophN ⊆ E → vπ ./ ζs →
   proph_ctx -∗ 1:[ξ] -∗ q:+[ζs] ={E}=∗ ⟨π, π ξ = vπ π⟩ ∗ q:+[ζs].
 Proof.
-  move: ξ vπ => [a[i inh]] vπ. set ξ := PrVar a (i, inh).
+  move: ξ vπ => [𝔄[i inh]] vπ. set ξ := PrVar 𝔄 (i, inh).
   iIntros (? Dep) "? Tok Ptoks". iInv prophN as (S) "> [(%L & %Ok & %Sim) Auth]".
   iDestruct (proph_tok_out with "Auth Tok") as %Outξ; [done|].
   set L' := .{ξ := vπ} :: L. iAssert ⌜∀ζ, ζ ∈ ζs → ζ ∉ res L'⌝%I as %Outζs.
@@ -356,16 +356,16 @@ Proof.
     by apply Eqv. }
   have InLNe ζ wπ : .{ζ := wπ} ∈ L → ξ ≠ ζ.
   { move=> /(elem_of_list_fmap_1 pli_pv) ??. by subst. }
-  move=> [b[j inh']] ?. rewrite elem_of_cons.
-  case (decide (ξ = PrVar b (j, inh')))=> [Eq|Ne].
+  move=> [𝔅[j inh']] ?. rewrite elem_of_cons.
+  case (decide (ξ = PrVar 𝔅 (j, inh')))=> [Eq|Ne].
   { move: (Eq)=> ?. dependent destruction Eq.
     rewrite /S' /add_line discrete_fun_lookup_insert lookup_insert. split.
     - move=> /(inj (Some ∘ aitem)) ->. left. by proof_subst inh' inh.
     - move=> [Eq'|/InLNe ?]; [|done]. proof_subst inh' inh.
       by dependent destruction Eq'. }
-  have Eqv : S' b !! j ≡ S b !! j.
+  have Eqv : S' 𝔅 !! j ≡ S 𝔅 !! j.
   { rewrite /S' /add_line /discrete_fun_insert.
-    case (decide (a = b))=> [?|?]; [|done]. simpl_eq.
+    case (decide (𝔄 = 𝔅))=> [?|?]; [|done]. simpl_eq.
     case (decide (i = j))=> [?|?]; [|by rewrite lookup_insert_ne]. subst.
     by proof_subst inh' inh. }
   rewrite Eqv Sim. split; [by right|]. move=> [Eq|?]; [|done].
@@ -374,7 +374,7 @@ Qed.
 
 (** Manipulating Prophecy Observations *)
 
-Implicit Type φπ ψπ: @proph TYPE Ty Prop.
+Implicit Type φπ ψπ: @proph _ Ty Prop.
 
 Lemma proph_obs_true φπ : (∀π, φπ π) → ⊢ ⟨π, φπ π⟩.
 Proof. move=> ?. iExists []. by iSplit. Qed.
@@ -399,12 +399,12 @@ Proof.
   iAssert ⌜π ◁ L'⌝%I as %?; last first.
   { iSplitL; last first. { iPureIntro. exists π. by apply SatTo. }
     iModIntro. iExists S. iFrame. iPureIntro. by exists L. }
-  rewrite /proph_sat Forall_forall. iIntros ([[a[i inh]] vπ] In)=>/=.
-  set ξ := PrVar a (i, inh). iAssert (proph_atom .{ξ := vπ}) with "[Atoms]" as "Atom".
+  rewrite /proph_sat Forall_forall. iIntros ([[𝔄[i inh]] vπ] In)=>/=.
+  set ξ := PrVar 𝔄 (i, inh). iAssert (proph_atom .{ξ := vπ}) with "[Atoms]" as "Atom".
   { iApply big_sepL_elem_of; by [apply In|]. }
   iDestruct (own_valid_2 with "Auth Atom") as %ValBoth. iPureIntro.
   move: ValBoth=> /auth_both_valid_discrete [Inc Val]. apply (Sat .{ξ := vπ}), Sim.
-  move/(discrete_fun_included_spec_1 _ _ a) in Inc.
+  move/(discrete_fun_included_spec_1 _ _ 𝔄) in Inc.
   rewrite /line discrete_fun_lookup_singleton in Inc.
   move: Inc=> /singleton_included_l [it [Eqv /Some_included [->|Inc]]]; [done|].
   rewrite Eqv. constructor. apply (lookup_valid_Some _ i it) in Val; [|done]. move: Val.
@@ -419,13 +419,8 @@ Global Opaque proph_ctx proph_tok proph_obs.
 
 (** * Prophecy Equalizer *)
 
-Section def.
-Context `{!invG Σ, !prophG TYPE Ty Σ}.
-
-Definition proph_eqz {A} (uπ vπ: _ → A) : iProp Σ :=
+Definition proph_eqz `{!invG Σ, !prophG TYPE Ty Σ} {A} (uπ vπ: _ → A) : iProp Σ :=
   ∀E ξs q, ⌜↑prophN ⊆ E ∧ vπ ./ ξs⌝ -∗ q:+[ξs] ={E}=∗ ⟨π, uπ π = vπ π⟩ ∗ q:+[ξs].
-
-End def.
 
 Notation "uπ :== vπ" := (proph_eqz uπ vπ) (at level 70, format "uπ  :==  vπ") : bi_scope.
 
